###### Shortcut
### $$g(x)=5x^2-8\Rightarrow g'(x)=10x^1-0\Rightarrow g'(x)=10x$$
###### Difference Quotients
### $$g(x=h)=5(x+h)^2-8$$
### $$g'(x)=\lim_{h\rightarrow0}\frac{g(x+h)-g(x)}{h}\Rightarrow g'(x)=\lim_{h\rightarrow0}\frac{[5(x+h)^2-8]-[5x^2-8]}{h}$$
 $$g'(x)=\lim_{h\rightarrow0}\frac{[5(x^2+h^2+xh)-8]-[5x^2-8]}{h}\Rightarrow g'(x)=\lim_{h\rightarrow0}\frac{[5x^2+5h^2+10xh-8]-[5x^2-8]}{h}$$
 $$g'(x)=\lim_{h\rightarrow0}\frac{5x^2+5h^2+10xh-8-5x^2+8}{h}\Rightarrow g'(x)=\lim_{h\rightarrow0}\frac{5h^2+10xh}{h}\Rightarrow g'(x)=\lim_{h\rightarrow0}\frac{h(5h+10x)}{h}$$
$$g'(x)=\lim_{h\rightarrow0}\frac{h(5h+10x)}{h}\Rightarrow g'(x)=\lim_{h\rightarrow0}5h+10x\Rightarrow g'(x)=5(0)+10x\Rightarrow g'(x)=10x$$

# Quiz 3 Calculus 1 Math 2210-12 James Wibowo
###### Q1
Using Difference Quotients find $f'(x)$:
$$f(x)=11$$
###### A1
$$f(x)=11\textrm{ and }f(x+h)=11$$
#### $$f'(x)=\lim_{h\rightarrow0}\frac{f(x+h)-f(x)}{h}\Rightarrow f'(x)=\lim_{h\rightarrow0}\frac{(11)-(11)}{h}\Rightarrow f'(x)=\lim_{h\rightarrow0}\frac{0}{h}\Rightarrow \boxed{f'(x)=0}$$
###### Q2
Using Difference Quotients find $f'(x)$:
$$f(x)=\sqrt{x}$$
###### A2
$$f(x)=x^{1/2}\textrm{ and }f(x+h)=(x+h)^{1/2}$$
$$f'(x)=\lim_{h\rightarrow0}\frac{f(x+h)-f(x)}{h}\Rightarrow f'(x)=\lim_{h\rightarrow0}\frac{\sqrt{x+h}-\sqrt{x}}{h}*\frac{\sqrt{x+h}+\sqrt{x}}{\sqrt{x+h}+\sqrt{x}}\Rightarrow f'(x)=\lim_{h\rightarrow0}\frac{x+h-x}{h(\sqrt{x+h}+\sqrt{x})}$$
$$f'(x)=\lim_{h\rightarrow0}\frac{h}{h(\sqrt{x+h}+\sqrt{x})}\Rightarrow f'(x)=\lim_{h\rightarrow0}\frac{1}{\sqrt{x+h}+\sqrt{x}}\Rightarrow f'(x)=\frac{1}{\sqrt{x}+\sqrt{x}}\Rightarrow \boxed{f'(x)=\frac{1}{2\sqrt{x}}}$$
$$(\sqrt{a}-\sqrt{b})(\sqrt{a}+\sqrt{b})=\frac{a-b}{\sqrt{a}+\sqrt{b}}$$
###### Q3
Using Difference Quotients find $f'(x)$:
$$f(x)=x^3+x$$
###### A3
$$f(x)=x^3+x\textrm{ and }f(x+h)=(x+h)^3+x+h$$
$$f'(x)=\lim_{h\rightarrow0}\frac{f(x+h)-f(x)}{h}\Rightarrow f'(x)=\lim_{h\rightarrow0}\frac{(x+h)^3+x+h-x^3+x}{h}\Rightarrow f'(x)=\lim_{h\rightarrow0}\frac{(x+h)^3+2x+h-x^3}{h}$$
$$f'(x)=\lim_{h\rightarrow0}\frac{(x+h)(x+h)(x+h)+2x+h-x^3}{h}\Rightarrow f'(x)=\lim_{h\rightarrow0}\frac{(x^2+h^2+2xh)(x+h)+2x+h-x^3}{h}$$
$$f'(x)=\lim_{h\rightarrow0}\frac{2x^2h+2h^2x+h^2x+h^3+2x+h-x^3}{h}\Rightarrow f'(x)=\lim_{h\rightarrow0}\frac{h(2x^2+2hx+hx+h^2)+2x-x^3}{h}$$
$$\lim_{h\rightarrow0}(2x^2+2hx+hx+h^2)+2x-x^3\Rightarrow f'(x)=(2x^2+2(0)x+(0)x+(0)^2)+2x-x^3\Rightarrow \boxed{f'(x)=3x^2+1}$$
	