# 6.4 Second Fundamental Theorem of Calculus
$\displaystyle \int_{a}^{b}{f(t)}dt=F(b)-F(a)$ where $F'(x)=f(x)$.
$\displaystyle\int_{a}^{x}{f(t)}dt=f(x)-F(a)$
ie: $\frac{d}{dx}\left(x^x-x\right)=\frac{d}{dx}\left(x^2\right)-\frac{d}{dx}\left(x\right)=2x-1$
$\Rightarrow\displaystyle\frac{d}{dx}\left(\int_{a}^{x}{f(t)}dt\right)=\frac{d}{dx}\left(f(x)-F(a)\right)$
$\Rightarrow\displaystyle\frac{d}{dx}\left(\int_{a}^{x}{f(t)}dt\right)=\frac{d}{dx}\left(F(x)\right)-\frac{d}{dx}\left(F(a)\right)$
$\Rightarrow\displaystyle\frac{d}{dx}\left(\int_{a}^{x}{f(t)}dt\right)=f(x)$
So $\displaystyle\int_{a}^{x}{f(t)}dt$ is an antiderivative of $f$

ie: $\frac{d}{dx}\left(\int_{-3}^{x}{t^2-2t}dt\right)=x^2-x$
$\frac{d}{dx}\left(\int_{\pi}^{x}{\sin{(t^2)}\cos{(t)}}dt\right)=\sin{(x^2)}\cos{(x)}$

TLDR: $\displaystyle\frac{d}{dx}\left(\int_{a}{x}{f(t)}dt\right)=f(x)$

`Hokora's TLDR: its a function to find the antiderivative of literally any function`

Let $\displaystyle F(x)=\int_{0}^{x}{e^{-t^2}}dt$
$\displaystyle\frac{d}{dx}\left(\frac{F(x)}{x}\right)=\frac{x\frac{d}{dx}\left(F(x)\right)-F(x)\frac{d}{dx}\left(x\right)}{x^2}$

> "Low dee high minus high dee low
> square the denominator down below"

$\displaystyle=\frac{xe^{-x^2}-F(x)}{x^2}=\frac{e^{-x^2}-\int_{0}^{x}e^{-t^2}}{x^2}$


$\displaystyle\frac{d}{dx}\left(\int_{0}^{x^2}{e^{-t^2}}dt\right)=\frac{d}{dx}\left(F(x^2)\right)$
$=F'(x^2)*\frac{d}{dx}\left(x^2\right)$
$\displaystyle e^{-(x^2)^2}(2x)$
$=2xe^{-x^4}$


Recall $\displaystyle\lim_{t\rightarrow0}{\frac{\sin{(t)}}{t}}=1$.
$\displaystyle f(t)=\biggr\{\begin{matrix}{\frac{\sin t}{t}}&{,t\ne0}\\{1}&{,t=0}\end{matrix}$
Scientists call
$Si(x)=\int_{0}^{x}{f(t)}dt$



Estimate: $Si(0),Si(1),Si(2),Si(3)$. using Riemann sums with $\Delta t=0.5$
$Si(0)=\int_{0}^{0}{\frac{\sin{(t)}}{dt}}dt=0$
$Si(1)=\int_{0}^{1}{\frac{\sin t}{t}}dt=$
! LHS: $f(0)*0.5+f(0.5)*0.5=\left(1*0.5\right)+\left(\left(\frac{\sin0.5}{0.5}\right)0.5\right)$
! RHS: $f(0.5)*0.5+f(1)*0.5=\left(\left(\frac{\sin0.5}{0.5}\right)0.5\right)+\left(\left(\frac{\sin1}{1}\right)0.5\right)$
! AVG: $(0.97945\dots+0.9002\dots)/2=0.94\dots$

$Si(2)=\int_{0}^{2}\frac{\sin t}{t}dt\approx1.60$
$Si(3)=\int_{0}^{3}\frac{\sin t}{t}dt\approx 1.84$

$\frac{d}{dx}(Si(x))=\frac{\sin x}{x}$



# 7.1 Integration by Substitution
$\frac{d}{dx}(sin(x^3))=\underbrace{\cos(x^3)}_{\text{derivative of outer function}}*\underbrace{3x^2}_{\text{derivative of inner function}}$
$\frac{d}{dx}(f(g(x))=f'(g(x))*g'(x)$
$\frac{d}{dx}(f(u))=f'(u)*\frac{du}{dx}$
$\int\frac{df}{dx}dx=\int\frac{df}{du}*\int\frac{du}{dx}dx$
$f(x)=\int f'(u)*\frac{du}{dx}dx=\int f'(u)du$
$\int f'(g(x))g'(x)dx=\int f'(u)du=f(u)+C=f(g(x))+C\rightarrow$
let $u=g(x)$
$\frac{du}{dx}=g'(x)$
$du=g'(x)dx$



$u=x^3$
$\frac{du}{dx}=3x^2$
$du=3x^2dx$
$\underset{=\int\cos()}{\int\cos}\underbrace{(x^3)}_{u}*\underbrace{3x^2dx}_{du}$
$=\sin(u)+C$
$=\sin(x^3)+C$


Ex: $\int x^3\sqrt{x^4+5}dx$

> $u=x^4+5$
> $\frac{du}{4}=\frac{4x^3dx}{4}$
> $\frac{1}{4}du=x^3dx$

$\displaystyle=\int \sqrt{4}(\frac{1}{4}du)$
$\displaystyle=\frac{1}{4}\int u^{\frac{1}{2}}du$
$\displaystyle=\frac{1}{4}\left(\frac{u^{\frac{3}{2}}}{\frac{3}{2}}\right)+C$
$\displaystyle=\frac{1}{2\xcancel{4}}*\frac{x^1}{3}u^{\frac{3}{2}}+C$
$\displaystyle=\frac{1}{6}\left(x^4+5\right)^{\frac{3}{2}}+C$


Ex: $\int e^{\cos\Theta}\sin\Theta d\Theta$

> $u=\cos\Theta$
> $du=-\sin\Theta d\Theta$
> $-du=\sin\Theta d\Theta$

$=\int e^u(-du)$
$=-\int e^udu$
$=-e^u+C$
$=-e^{\cos\Theta}+C$



Ex: $\int\frac{e^t}{1+e^t}dt$
$=\int\frac{e^tdt}{1+e^t}=\int\frac{du}{u}$

> $u=1+e^t$
> $du=e^tdt$

$=\int\frac{1}{u}du$
$=\ln|u|+C$
$=\ln|1+e^t|+C$
$=\ln(1+e^t)+C$

$\frac{d}{dt}(\ln(1+e^t))=\frac{1}{1+e^t}(1+e^t)'=\frac{e^t}{1+e^t}$


Ex: $\int\tan\Theta d\Theta=\int\frac{\sin\Theta}{\cos\Theta}d\Theta$

> $\xcancel{\begin{matrix}u=\sin\Theta \\ du=\cos\Theta d\Theta\end{matrix}}$
> $u=\cos\theta$
> $du=-\sin\Theta d\Theta$
> $-du=\sin\Theta d\Theta$

$=\int\frac{-du}{u}$
$=\int-\frac{1}{u}du$
$=-\ln|u|+C$
$=-\ln|\cos\Theta|+C$



Ex: $\int e^x\cos^3(e^x)\sin(e^x)dx$

> $u=e^x$
> $du=e^xdx$

$=\int\underbrace{\cos^3(u)}_{(\cos u)^3}\sin(u)du$

> $w=cosu$
> $dw=\sin(u)du$
> $-dw=sin(u)du$

$\displaystyle=\int-w^3dw=-\frac{w^4}{4}+C=\frac{\cos^4u}{4}+C=-\frac{\cos^4(e^x)}{4}+C$

Second way of doing it:

$\int e^x\cos^3(e^x)\sin(e^x)dx$

> $u=\cos(e^x)$
> $du=-\sin(e^x)(e^x)dx$
> $-du=\sin(e^x)e^xdx$

$=\int u^3(-du)=-\frac{u^4}{4}+C$
$=-\frac{\cos^4(e^x)}{4}+C$


Ex:$\int_{0}^{2}xe^{x^2}dx$

> $u=x^2$
> $\underset{2}{\underline{du}}=\underset{2}{\underline{2xdx}}$
> $\frac{du}{2}=xdx$

$=\int_{0}^{2}e^u$
$=\frac{1}{2}\int_{x=0}^{x=2}e^udu$
$=\frac{1}{2}\int_{x=0}^{x=2}e^udu$
$\xcancel{\begin{matrix}{=\frac{1}{2}e^u\biggr|_{0}^{2}} \\ {=\frac{1}{2}e^2-\frac{1}{2}e^0} \\ {=\frac{1}{2}e^2-\frac{1}{2}}\end{matrix}}$

$\int xe^{x^2}dx$

> $u=x^2$
> $\frac{du}{2}=xdx$

$=\frac{1}{2}\int e^udu$
$=\frac{1}{2}e^u+C$
$=\frac{1}{2}e^{x^2}+C$
