Ex: $\displaystyle\int\frac{x}{(x^2+1)^2}dx$
> $u=(x^2+1)^2$


##### power rule for antiderivative
$\displaystyle\int x^ndx=\frac{n^{n+1}}{n+1}+C$


$\int_{0}^{2}xe^{x^2}dx$
> $u=x^2$
> $du=2xdx$
> $\frac{1}{2}du=xdx$

$=\int_{0}^{2}e^{x^2}xdx$
$=\int_{x=0}^{x=2}e^u\left(\frac{1}{2}du\right)$
$=\frac{1}{2}\int_{x=0}^{x=2}e^udu$
$=\frac{1}{2}e^u\biggr|_{x=0}^{x=2}$
$=\frac{1}{2}e^{x^2}\biggr|_{0}^{2}$
$=\frac{1}{2}e^{2^2}-\frac{1}{2}e^0$
$\frac{1}{2}e^4-\frac{1}{2}$

OR

$=\int_{0}^{4}e^u\left(\frac{1}{2}du\right)$
$=\frac{1}{2}\int_{0}^{4}e^udu$
$=\frac{1}{2}e^u\biggr|_{0}^{4}$
$\frac{1}{2}e^4-\frac{1}{2}e^0$
$\frac{1}{2}e^4-\frac{1}{2}$


# $u$-subs for Definite Integrals
## Method 1:
Find antiderivative in terms of original variable, then plug in original bounds of integration
## Method 2:
After $u$-sub, find new bounds in terms of $u$, then do not convert antiderivatives back to original variable.

Ex:
$\int_{1}^{2}\frac{x}{(x^2+1)^2}dx$
> $u=x^2+1$
> $du=2xdx$
> $\frac{1}{2}du-xdx$

$=\int_{1}^{2}\frac{1}{u^2}(\frac{1}{2}du)$
$=\frac{1}{2}\int\frac{1}{u^2}du$


$=\int_{2}^{5}\frac{1}{u^2}(\frac{1}{2}du)$
$=\frac{1}{2}\int_{2}^{5}\frac{1}{u^2}du$
$=\frac{1}{2}\int_{2}^{5}$

using method 2:
> u=x^2+1
> $x=1:u=1^2+1=2$
> $x=2:u=2^2+1=5$

$=\int_{x=1}^{x=2}\frac{1}{u^2}\left(\frac{1}{2}du\right)$
$\frac{1}{2}\int_{x=1}^{x=2}u^{-2}du$

`hokora please finish this later im so tired i need to catch up with the notes thanks`


Ex: $\int\sqrt{1+\sqrt x}dx$
> $u=1+\sqrt x$
> $u=1+x^{\frac{1}{2}}$
> $du=\frac{1}{2}x^{-\frac{1}{2}}dx$
>>what if i solve for $x$ instead?
>>$u-1=\sqrt x$
>>$(u-1)^2=x$
>>2(u-1)du=dx

$=\int\sqrt udx$
$=\int\sqrt u(2)(u-1)du$
$=2\int u^{\frac{1}{2}}\left(u^{\frac{2}{2}}-1\right)du$
$=2\int u^{\frac{3}{2}}-u^{\frac{1}{2}}du$
$\displaystyle=2\left(\frac{u^{\frac{5}{2}}}{\frac{5}{2}}-\frac{u^{\frac{3}{2}}}{\frac{3}{2}}\right)+C$
$\displaystyle=2\left(\frac{2}{5}u^{\frac{5}{2}}-\frac{2}{3}u^{\frac{3}{2}}\right)$
$\displaystyle=2\left(\frac{2}{5}\left(1+\sqrt{x}\right)^{\frac{5}{2}}-\frac{2}{3}\left(1+\sqrt{x}\right)^{\frac{3}{2}}\right)+C$



Ex: $\displaystyle\int(x+7)\sqrt[3]{3-2x}dx$
> $\int(x+7)\sqrt[3]{x}dx$
> $\int\left(x^1+7\right)x^{\frac{1}{3}}dx$
> $\int x^{\frac{4}{3}}+7x^{\frac{1}{2}}dx$
> $\displaystyle\frac{x^{\frac{7}{3}}}{\frac{7}{3}}+7\frac{x^{\frac{4}{3}}}{\frac{4}{3}}+C$

$=\int(x+7)(3-2x)^{\frac{1}{3}}dx$

> $u=3-2x$
> $du=-2dx$
> $-\frac{1}{2}du=dx$
> $u=3-2x$
> $u-3=-2x$
> $\frac{3-u}{2}=x$

$=\int(x+7)u^{\frac{1}{3}}dx$
$=\int(x+7)u^{\frac{1}{3}}\left(-\frac{1}{2}\right)du$
$=\int\left(\frac{3-u}{2}+7\right)u^{\frac{1}{3}}\left(-\frac{1}{2}\right)du$
$=\int\left(\frac{3}{2}-\frac{u}{2}+\frac{14}{2}\right)u^{\frac{1}{3}}\left(-\frac{1}{2}\right)du$
$=\int\left(\frac{17}{2}-\frac{u}{2}\right)u^{\frac{1}{3}}\left(-\frac{1}{2}\right)du$
$=-\frac{1}{2}\int\frac{17}{2}u^{\frac{1}{3}}-\frac{u^{\frac{4}{3}}}{7}du$
$\displaystyle=-\frac{1}{2}\left(\frac{17}{2}*\frac{u^{\frac{1}{3}}}{\frac{4}{3}}-\frac{u^{\frac{4}{3}}}{2*\frac{7}{3}}\right)+C$


Ex:$\int_{-1}^{1}\sqrt{x+1}dx$

>$u=x+1$






Ex: $\int x\sqrt{x+1}dx$

