# 7.2 Integration by Parts

Product Rule
$\displaystyle\frac{d}{dx}(uv)=v\frac{du}{dx}+u\frac{du}{dx}$
$\displaystyle\int\frac{d}{dx}(uv)dx=\int\left(v\frac{du}{dx}+u\frac{du}{dx}\right)dx$
$uv=\int v\frac{du}{dx}dx+\int u\frac{du}{dx}dx$
$uv=\int vdu+\int udv$
$uv-\int vdu=\int udv$

## Integration by parts
$\int udv=uv-\int vdu$
$\int_a^vudv=uv\biggr|_a^b-\int_a^bvud$

###### Ex:
Find $\int xe^xdx$
> $u=x$
> $du=dx$

> $dv=e^xdx$
> $\int dv=\int e^xdx$
> $v=e^x$

$\int xe^xdx=xe^x-\int e^xdx$
$x-e^x+C$

> $u=x$
> $du=dx$

> $dv=e^xdx$
> $v=e^x$

Check:
$(xe^x-e^x+C)'=(xe^x)'-(e^x)'+C'$
$=x'e^x+(e^x)'-e^x+0$
$=\cancel{e^x}+xe^x-\cancel{e^x}$
$=xe^x$


> $u=e^x$
> $du=e^xdx$

> $dv=xdx$
> $\int dv=\int x^1dx$
> $v=\frac{x^2}{2}$

$\int xe^xdx=e^x(\frac{x^2}{2})-\int\frac{x^2}{2}e^xdx$



###### Ex:
$\int\theta\cos\theta d\theta$

> $u=\theta$
> $du=d\theta$

> $dv=cos\theta d\theta$
> $\int dv=\int\cos\theta d\theta$
> $v=\sin\theta$

$\int\theta\cos\theta d\theta=\theta\sin\theta-\int\sin\theta d\theta$
$=\sin\theta-(-\cos\theta)+C$
$=\theta\sin\theta+\cos\theta+C$

#### How to choose $u$ and $dv$?
- Whatever you pick $du$ to be, you should be able to find its antiderivative $v$.
- It helps if $du$ is simpler than $u$ (or at the very least, not more complicated).
- It helps if $v$ is simpler than $dv$ (or at the very least, not more complicated).


###### Ex:
$\int_2^3\ln xdx$

> $u=\ln x$
> $du=\frac1xdx$

> $dv=dx$
> $\int dv=\int dx$
> $v=x$

$\displaystyle\int_2^3\ln xdx=(\ln x)(x)\biggr|_2^3-\int_2^3x*\frac1xdx$
$=x\ln x\biggr|_2^3-\int_2^31dx$
$=x\ln x-x\biggr|_2^3$
$=3\ln3-3-(2\ln2-2)$
$=3\ln3-3-2\ln2+2$
$=3\ln3-2\ln2-1$

###### Ex:
$\int x^6\ln xdx$

> $u=\ln x$
> $du=\frac1xdx$

> $dv=x^6dx$
> $\int dv=\int dx^6dx$
> $v=\frac {x^7}7$

$\ln x\left(\frac{x^7}7\right)-\int\frac{x^{\cancel7\fbox6}}7*\frac1{\cancel x}dx$
$=\frac{x^7}7\ln x-\int\frac{x^6}7dx$
$=\frac{x^7}7\ln x-\int\frac17x^6dx$
$=\frac{x^7}7\ln x-\frac17\left(\frac{x^7}7\right)+C$
$\frac{x^7}7\ln x-\frac{x^7}{49}+C$




(shortcut noted here)


$\int\sin(-3x+7)dx$
$=\frac1{\cancel{-}+3}(\cancel{-}+\cos(-3x+7))+C$
$=\frac13\cos(-3x+7)+C$



$f(x)$
$f'(x)=\frac{df}{dx}$

$f'(x)*dx=\frac{df}{dx}*dx$
$f'(x)dx=df$
###### Ex:
$\int x^2\sin4xdx$

> $u=x^2$
> $du=2xdx$
> ($\frac{du}{dx}=2x$)

> $dv=\sin4xdx$
> $\int dv=\int\sin4xdx$
> $v=-\frac14\cos4x$

$=x^2\left(-\frac14\cos4x\right)-\int-\frac14\cos(4x)2xdx$
$=x^2\left(-\frac14\cos4x\right)+\int+\frac14\cos(4x)2xdx$
$=-\frac14x^2\cos4x+\frac12\int\cos(4x)xdx$

> $u=x$
> $du=dx$

> $dv=\cos(4x)dx$
> $\int dv=\int\cos(4x)dx$
> $v=\frac14\sin(4x)$

$\displaystyle=-\frac14x^2\cos4x+\frac12\left(x\left(\frac14\sin(4x)\right)-\int\frac14\sin(4x)dx\right)$
$\displaystyle=-\frac14x^2\cos4x+\frac12\left(\frac14x\sin4x+\frac14\left(+\frac14\cos(4x)\right)\right)+C$
$\displaystyle=-\frac14x^2\cos4x+\frac12\left(\frac14x\sin4x+\frac1{16}\cos4x\right)+C$
$\text{Final Answer:}\displaystyle=-\frac14x^2\cos4x+\frac18x\sin4x+\frac1{32}\cos4x+C$


###### Ex:
$\int\cos^2\theta d\theta=\int(\cos\theta)^2d\theta$

> $u=\cos\theta$
> $du=-\sin\theta d\theta$
> u-sub doesn't work

$\int\cos\theta\cos\theta d\theta$

> $u=\cos\theta$
> $du=-\sin\theta d\theta$

> $dv=\cos\theta d\theta$
> $\int dv=\int\cos\theta d\theta$
> $v=\sin\theta$

$=\cos\theta\sin\theta-\int\sin\theta(-\sin\theta d\theta)$
$=\cos\theta\sin\theta+\int\sin\theta(+\sin\theta d\theta)$
$=\cos\theta\sin\theta+\int\underbrace{\sin^2\theta}_{\text{read below}} d\theta$

> $\sin^2\theta+\cos^2\theta=1$
> $\sin^2\theta=1-\cos^2\theta$

$=\cos\theta\sin\theta+\int1-\cos^2\theta d\theta=\cos\theta\sin\theta+\int1d\theta-\int\cos^2\theta d\theta$
$=cos\theta\sin\theta+\theta-\int\cos^2\theta d\theta$
$\underbrace{\int\cos^2\theta d\theta}_{+\int\cos^2\theta d\theta}=\cos\theta\sin\theta+\theta\underbrace{-\int\cos^2\theta d\theta}_{+\int\cos^2\theta d\theta}$
$2\int\cos^2\theta d\theta=\cos\theta\sin\theta+\theta+C$
$\frac12*2\int\cos^2\theta d\theta=\left(\cos\theta\sin\theta+\theta+C\right)\frac12$
$\int\cos^2\theta d\theta=\frac12\cos\theta\sin\theta+\frac12\theta+C$


###### Ex:
$\int e^x\sin xdx$

> $u=e^x$
> $du-e^xdx$

> $dv=\sin xdx$
> $\int dv=\int\sin xdx$
> $v=-\cos x$

$=e^x(-\cos x)-\int-\cos xe^xdx$
$=e^x(-\cos x)+\int+\cos xe^xdx$
$=$